ExistentialRules/ChaseSequence/CoreChase/CoreChaseNode.lean
@@ -1,30 +1,50 @@
-import ExistentialRules.ChaseSequence.ChaseBranch
-import ExistentialRules.Models.Basic
-import ExistentialRules.Models.Cores
-import PossiblyInfiniteTrees.PossiblyInfiniteTree.FiniteDegreeTree.Basic
-import ExistentialRules.Models.Basic
-import ExistentialRules.Triggers.Basic
-import ExistentialRules.AtomsAndFacts.Basic
-import ExistentialRules.AtomsAndFacts.SubstitutionsAndHomomorphisms
-import ExistentialRules.ChaseSequence.Termination.Basic
-import ExistentialRules.ChaseSequence.Universality
+/-
+Copyright 2026 Henrik Tscherny, Lukas Gerlach
+Released under Apache 2.0 license as described in the file LICENSE.
+-/
 
-import ExistentialRules.ChaseSequence.Deterministic
+module
+
+public import ExistentialRules.Models.Cores
+public import ExistentialRules.ChaseSequence.ChaseNode
+
+/-!
+# Core Chase Node
+
+Similar to a `ChaseNode`, we define another elements of the core chase in a similar fashion.
+Besides fact set and origin, these also store the core that the fact set is being condensed to. In principle any such core is allowed and we do not enforce a specific computation procedure.
+-/
+
+public section
 
 variable {sig : Signature} [DecidableEq sig.P] [DecidableEq sig.C] [DecidableEq sig.V]
 
+/-- The CoreChaseNode add a couple of fields on top of the RegularChaseNode but the `facts` field has a different meaning. This is why we duplicate the structure and not jsut extend it. We want to prevent that the `CoreChaseNode` is accidentally treated as a `RegularChaseNode`. -/
 structure CoreChaseNode (rules : RuleSet sig) where
-  fs : FactSet sig
+  facts : FactSet sig
+  origin : Option ((trg : RTrigger (RestrictedObsolescence sig) rules) × Fin trg.val.mapped_head.length)
+  facts_contain_origin_result : ∀ orig ∈ origin, orig.fst.val.mapped_head[orig.snd.val].toSet ⊆ facts
   core : FactSet sig
-  is_core : core.isWeakCore
-  core_sse : core.homSubset fs
-  origin : Option ((trg : RTrigger (RestrictedObsolescence sig).toLaxObsolescenceCondition rules) × Fin trg.val.mapped_head.length)
-  fs_contains_origin_result : ∀ o ∈ origin, o.fst.val.mapped_head[o.snd.val].toSet ⊆ fs
+  isWeakCore : core.isWeakCore
+  homSubset : core.homSubset facts
 
 namespace CoreChaseNode
 
-def origin_result {rules : RuleSet sig} (node : CoreChaseNode rules) (isSome : node.origin.isSome) : List (Fact sig) :=
-  let origin := node.origin.get isSome
-  origin.fst.val.mapped_head[origin.snd.val]
+variable {rules : RuleSet sig}
+
+/-- The `CoreChaseNode` is a `ChaseNode` where the outgoingFacts are a core of the ingoingFacts. -/
+instance coreChaseNodeInstance : ChaseNode (CoreChaseNode rules) (RestrictedObsolescence sig) rules where
+  ingoingFacts := CoreChaseNode.facts
+  outgoingFacts := CoreChaseNode.core
+  origin := CoreChaseNode.origin
+  facts_contain_origin_result := CoreChaseNode.facts_contain_origin_result
+
+theorem ingoingFacts_eq {node : CoreChaseNode rules} : coreChaseNodeInstance.ingoingFacts node = node.facts := by rfl
+theorem outgoingFacts_eq {node : CoreChaseNode rules} : coreChaseNodeInstance.outgoingFacts node = node.core := by rfl
+
+/-- The `CoreChaseNode` has the `ChaseNode.out_sub_in` property. -/
+theorem out_sub_in : coreChaseNodeInstance.out_sub_in (N := CoreChaseNode rules) := by
+  intro node f; rw [ingoingFacts_eq, outgoingFacts_eq]; exact node.homSubset.left f
 
 end CoreChaseNode
+
